first pass through bucketiterator

lib/Buckets/BucketIteratorModel.i.dfy
@@ -2,9 +2,10 @@
 // SPDX-License-Identifier: BSD-2-Clause
 
 include "BucketsLib.i.dfy"
+include "TranslationLib.i.dfy"
 include "../Base/Sets.i.dfy"
 //
-// A mathematical description of bucket iterators.
+// A mathematical description of bucket iterators for successor query.
 // The implementation is defined in BucketImpl together with MutBucket.
 //
 
@@ -17,19 +18,52 @@ module BucketIteratorModel {
   import opened Sequences
   import opened KeyType
   import opened BucketMaps
+  import opened TranslationLib
   import MapSeqs
 
   datatype IteratorOutput = Next(key: Key, msg: Message) | Done
 
   datatype Iterator = Iterator(
+    pset: Option<PrefixSet>,
     ghost next: IteratorOutput,
     ghost idx: int,
     ghost decreaser: int
-  ) 
+  )
 
   function SetGte(bucket: BucketMap, key: Key) : set<Key>
   {
     set k | k in bucket && Keyspace.lte(key, k)
+  }
+
+  function SuccBucket(bucket: Bucket, pset: Option<PrefixSet>): Bucket
+  requires PreWFBucket(bucket)
+  {
+    if pset.None? then bucket else TranslateBucket(bucket, pset.value.prefix, pset.value.newPrefix)
+  }
+
+  function SuccIdx(bucket: Bucket, pset: Option<PrefixSet>, idx: int): (i: int)
+  requires PreWFBucket(bucket)
+  requires 0 <= idx < |bucket.keys|
+  requires pset.Some? ==> IsPrefix(pset.value.prefix, bucket.keys[idx])
+  ensures 0 <= i < |SuccBucket(bucket, pset).keys|
+  ensures SuccBucket(bucket, pset).keys[i] == ApplyPrefixSet(pset, bucket.keys[idx])
+  {
+    if pset.None? then idx else (
+      var tbucket := TranslateBucketInternal(bucket, pset.value.prefix, pset.value.newPrefix, 0);
+      var i :| 0 <= i < |tbucket.idxs| && tbucket.idxs[i] == idx;
+      i
+    )
+  }
+
+  predicate WFIterNext(bucket: Bucket, it: Iterator)
+  requires PreWFBucket(bucket)
+  requires it.next.Next?
+  {
+    && it.decreaser > 0
+    && 0 <= it.idx < |bucket.keys|
+    && (it.pset.Some? ==> IsPrefix(it.pset.value.prefix, bucket.keys[it.idx]))
+    && it.next.key == ApplyPrefixSet(it.pset, bucket.keys[it.idx])
+    && it.next.msg == bucket.msgs[it.idx]
   }
 
   predicate {:opaque} WFIter(bucket: Bucket, it: Iterator)
@@ -37,8 +71,8 @@ module BucketIteratorModel {
       && PreWFBucket(bucket)
       && it.decreaser >= 0
       && (it.next.Next? && BucketWellMarshalled(bucket) ==> (
-        && it.next.key in bucket.as_map()
-        && bucket.as_map()[it.next.key] == it.next.msg
+        && it.next.key in SuccBucket(bucket, it.pset).as_map()
+        && it.next.msg == SuccBucket(bucket, it.pset).as_map()[it.next.key]
       ))
   {
     && PreWFBucket(bucket)
@@ -46,38 +80,32 @@ module BucketIteratorModel {
     && it.idx >= 0
     && it.idx + it.decreaser == |bucket.keys|
     && |bucket.keys| == |bucket.msgs|
-    && (it.next.Next? ==> (
-      && it.decreaser > 0
-      && it.next.key == bucket.keys[it.idx]
-      && it.next.msg == bucket.msgs[it.idx]
-    ))
-    && (it.next.Done? ==> (
-      && it.decreaser == 0
-    ))
+    && (it.next.Next? ==> WFIterNext(bucket, it))
+    && (it.next.Done? ==> it.decreaser == 0)
     && (it.next.Next? && BucketWellMarshalled(bucket) ==> (
-      && it.next.key in bucket.as_map()
-      && bucket.as_map()[it.next.key] == it.next.msg
+        && it.next.key in SuccBucket(bucket, it.pset).as_map()
+        && it.next.msg == SuccBucket(bucket, it.pset).as_map()[it.next.key]
     ))
   }
 
-  function iterForIndex(bucket: Bucket, idx: int) : (it: Iterator)
-  requires WFBucket(bucket)
-  requires |bucket.keys| == |bucket.msgs|
+  function iterForIndex(bucket: Bucket, pset: Option<PrefixSet>,  idx: int) : (it: Iterator)
+  requires PreWFBucket(bucket)
   requires 0 <= idx <= |bucket.keys|
+  requires idx < |bucket.keys| && pset.Some? ==> IsPrefix(pset.value.prefix, bucket.keys[idx])
   ensures WFIter(bucket, it)
   {
     reveal WFIter();
 
-    var it := Iterator(
-      (if idx == |bucket.keys| then Done
-          else Next(bucket.keys[idx], bucket.msgs[idx])),
-      idx,
-      |bucket.keys| - idx);
+    var next := if idx == |bucket.keys| then Done else Next(ApplyPrefixSet(pset, bucket.keys[idx]), bucket.msgs[idx]);
 
+    var it := Iterator(pset, next, idx, |bucket.keys| - idx);
     assert (it.next.Next? && BucketWellMarshalled(bucket) ==> (
-      MapSeqs.MapMapsIndex(bucket.keys, bucket.msgs, idx);
-      && it.next.key in bucket.as_map()
-      && bucket.as_map()[it.next.key] == it.next.msg
+      var succidx := SuccIdx(bucket, pset, idx);
+      var succbucket := SuccBucket(bucket, pset);
+
+      MapSeqs.MapMapsIndex(succbucket.keys, succbucket.msgs, succidx);
+      && it.next.key in succbucket.as_map()
+      && it.next.msg == succbucket.as_map()[it.next.key]
     ));
     it
   }
@@ -87,36 +115,61 @@ module BucketIteratorModel {
   ensures WFIter(bucket, it)
   {
     reveal WFIter();
-    Iterator(Done, |bucket.keys|, 0)
+    Iterator(None, Done, |bucket.keys|, 0)
   }
 
   ///// Functions for initializing and manipulating iterators
 
-  function {:opaque} IterStart(bucket: Bucket) : (it' : Iterator)
+  // linear search
+  function iterNextWithPrefix(bucket: Bucket, prefix: Key, idx: int) : (i: int)
+  requires PreWFBucket(bucket)
+  requires 0 <= idx <= |bucket.keys|
+  ensures idx <= i <= |bucket.keys|
+  ensures i < |bucket.keys| ==> IsPrefix(prefix, bucket.keys[i])
+  ensures forall j | idx <= j < i :: !IsPrefix(prefix, bucket.keys[j])
+  decreases |bucket.keys| - idx
+  {
+    if idx < |bucket.keys| && !IsPrefix(prefix, bucket.keys[idx]) then (
+      iterNextWithPrefix(bucket, prefix, idx+1)
+    ) else (
+      idx
+    )
+  }
+
+  function {:opaque} IterStart(bucket: Bucket, pset: Option<PrefixSet>) : (it' : Iterator)
   requires WFBucket(bucket)
   ensures WFIter(bucket, it')
   {
     reveal WFIter();
-    iterForIndex(bucket, 0)
+
+    var i := if pset.None? then 0 else iterNextWithPrefix(bucket, pset.value.prefix, 0);
+    iterForIndex(bucket, pset, i)
   }
 
-  function {:opaque} IterFindFirstGte(bucket: Bucket, key: Key) : (it' : Iterator)
+  function {:opaque} IterFindFirstGte(bucket: Bucket, pset: Option<PrefixSet>, key: Key) : (it' : Iterator)
   requires WFBucket(bucket)
+  // requires pset.Some? ==> IsPrefix(pset.value.prefix, key)
   ensures WFIter(bucket, it')
-  ensures it'.next.Next? ==> Keyspace.lte(key, it'.next.key)
+  // ensures it'.next.Next? ==> Keyspace.lte(ApplyPrefixSet(pset, key), it'.next.key)
+  // ^ can't make this promise without bucketmarshalled.
   {
-    iterForIndex(bucket,
-      Keyspace.binarySearchIndexOfFirstKeyGte(bucket.keys, key))
+    var start := Keyspace.binarySearchIndexOfFirstKeyGte(bucket.keys, key);
+    var i := if pset.None? then start else iterNextWithPrefix(bucket, pset.value.prefix, start);
+    iterForIndex(bucket, pset, i)
   }
 
-  function {:opaque} IterFindFirstGt(bucket: Bucket, key: Key) : (it' : Iterator)
+  function {:opaque} IterFindFirstGt(bucket: Bucket, pset: Option<PrefixSet>, key: Key) : (it' : Iterator)
   requires WFBucket(bucket)
+  // requires pset.Some? ==> IsPrefix(pset.value.prefix, key)
   ensures WFIter(bucket, it')
-  ensures it'.next.Next? ==> Keyspace.lt(key, it'.next.key)
+  // ensures it'.next.Next? ==> Keyspace.lt(key, it'.next.key)
+  // ^ ditto
   {
     reveal WFIter();
-    iterForIndex(bucket,
-      Keyspace.binarySearchIndexOfFirstKeyGt(bucket.keys, key))
+
+    var start := Keyspace.binarySearchIndexOfFirstKeyGt(bucket.keys, key);
+    var i := if pset.None? then start else iterNextWithPrefix(bucket, pset.value.prefix, start);
+    iterForIndex(bucket, pset, i)
   }
 
   function {:opaque} IterInc(bucket: Bucket, it: Iterator) : (it' : Iterator)
@@ -127,7 +180,9 @@ module BucketIteratorModel {
   ensures it'.decreaser < it.decreaser
   {
     reveal WFIter();
-    iterForIndex(bucket, it.idx + 1)
+
+    var i := if it.pset.None? then it.idx+1 else iterNextWithPrefix(bucket, it.pset.value.prefix, it.idx+1);
+    iterForIndex(bucket, it.pset, i)
   }
 
   lemma noKeyBetweenIterAndIterInc(bucket: Bucket, it: Iterator, key: Key)
@@ -135,16 +190,35 @@ module BucketIteratorModel {
   requires BucketWellMarshalled(bucket)
   requires WFIter(bucket, it)
   requires key in bucket.as_map()
+  requires it.pset.Some? ==> IsPrefix(it.pset.value.prefix, key)
+  // requires key in SuccBucket(bucket, it.pset).as_map()
   requires it.next.Next?
   ensures IterInc(bucket, it).next.Next? ==>
-      (Keyspace.lte(key, it.next.key) || Keyspace.lte(IterInc(bucket, it).next.key, key))
+      ( Keyspace.lte(ApplyPrefixSet(it.pset, key), it.next.key) 
+     || Keyspace.lte(IterInc(bucket, it).next.key, ApplyPrefixSet(it.pset, key)))
   ensures IterInc(bucket, it).next.Done? ==>
-      Keyspace.lte(key, it.next.key)
+      Keyspace.lte(ApplyPrefixSet(it.pset, key), it.next.key)
   {
     reveal WFIter();
     Keyspace.reveal_IsStrictlySorted();
     reveal_IterInc();
-    var i := MapSeqs.GetIndex(bucket.keys, bucket.msgs, key);
+
+    var idx := MapSeqs.GetIndex(bucket.keys, bucket.msgs, key);
+    var key' := ApplyPrefixSet(it.pset, key);
+
+    if it.pset.Some? {
+      var itinc := IterInc(bucket, it);
+      assert idx <= it.idx || itinc.idx <= idx;
+      if idx <= it.idx {
+        PrefixLteProperties(it.pset.value.prefix, key, bucket.keys[it.idx]);
+        PrefixLteProperties(it.pset.value.newPrefix, key', it.next.key);
+        assert Keyspace.lte(key', it.next.key);
+      } else {
+        PrefixLteProperties(it.pset.value.prefix, bucket.keys[itinc.idx], key);
+        PrefixLteProperties(it.pset.value.newPrefix, itinc.next.key, key');
+        assert Keyspace.lte(itinc.next.key, key');
+      }
+    }
   }
 
   lemma IterIncKeyGreater(bucket: Bucket, it: Iterator)
@@ -158,46 +232,79 @@ module BucketIteratorModel {
     reveal WFIter();
     Keyspace.reveal_IsStrictlySorted();
     reveal_IterInc();
+
+    var itinc := IterInc(bucket, it);
+    if itinc.next.Next? && it.pset.Some? {
+      PrefixLteProperties(it.pset.value.prefix, bucket.keys[it.idx], bucket.keys[itinc.idx]);
+      PrefixLteProperties(it.pset.value.newPrefix, it.next.key, itinc.next.key);
+    }
   }
 
-  lemma noKeyBetweenIterFindFirstGte(bucket: Bucket, key: Key, key0: Key)
+  // TODO: is keyspace.lt(key0, key) still good ensures?
+  lemma noKeyBetweenIterFindFirstGte(bucket: Bucket, pset: Option<PrefixSet>, key: Key, key0: Key)
   requires WFBucket(bucket)
   requires BucketWellMarshalled(bucket)
   requires key0 in bucket.as_map()
-  ensures IterFindFirstGte(bucket, key).next.Next? ==>
-      (Keyspace.lt(key0, key) || Keyspace.lte(IterFindFirstGte(bucket, key).next.key, key0))
-  ensures IterFindFirstGte(bucket, key).next.Done? ==>
+  requires pset.Some? ==> IsPrefix(pset.value.prefix, key0)
+  ensures IterFindFirstGte(bucket, pset, key).next.Next? ==>
+      (Keyspace.lt(key0, key) || Keyspace.lte(IterFindFirstGte(bucket, pset, key).next.key, ApplyPrefixSet(pset, key0)))
+  ensures IterFindFirstGte(bucket, pset, key).next.Done? ==>
       (Keyspace.lt(key0, key))
   {
     Keyspace.reveal_IsStrictlySorted();
     reveal_IterFindFirstGte();
     var i := MapSeqs.GetIndex(bucket.keys, bucket.msgs, key0);
+    var itgte := IterFindFirstGte(bucket, pset, key);
+
+    if itgte.next.Next? && itgte.idx <= i && pset.Some? {
+      var key0' := ApplyPrefixSet(pset, key0);
+      PrefixLteProperties(pset.value.prefix, bucket.keys[itgte.idx], key0);
+      PrefixLteProperties(pset.value.newPrefix, itgte.next.key, key0');
+      assert Keyspace.lte(itgte.next.key, key0');
+    }
   }
 
-  lemma noKeyBetweenIterFindFirstGt(bucket: Bucket, key: Key, key0: Key)
+  lemma noKeyBetweenIterFindFirstGt(bucket: Bucket, pset: Option<PrefixSet>, key: Key, key0: Key)
   requires WFBucket(bucket)
   requires BucketWellMarshalled(bucket)
   requires key0 in bucket.as_map()
-  ensures IterFindFirstGt(bucket, key).next.Next? ==>
-      (Keyspace.lte(key0, key) || Keyspace.lte(IterFindFirstGt(bucket, key).next.key, key0))
-  ensures IterFindFirstGt(bucket, key).next.Done? ==>
+  requires pset.Some? ==> IsPrefix(pset.value.prefix, key0)
+  ensures IterFindFirstGt(bucket, pset, key).next.Next? ==>
+      (Keyspace.lte(key0, key) || Keyspace.lte(IterFindFirstGt(bucket, pset, key).next.key, ApplyPrefixSet(pset, key0)))
+  ensures IterFindFirstGt(bucket, pset, key).next.Done? ==>
       (Keyspace.lte(key0, key))
   {
     Keyspace.reveal_IsStrictlySorted();
     reveal_IterFindFirstGt();
     var i := MapSeqs.GetIndex(bucket.keys, bucket.msgs, key0);
+    var itgt := IterFindFirstGt(bucket, pset, key);
+
+    if itgt.next.Next? && itgt.idx <= i && pset.Some? {
+      var key0' := ApplyPrefixSet(pset, key0);
+      PrefixLteProperties(pset.value.prefix, bucket.keys[itgt.idx], key0);
+      PrefixLteProperties(pset.value.newPrefix, itgt.next.key, key0');
+      assert Keyspace.lte(itgt.next.key, key0');
+    }
   }
 
-  lemma noKeyBeforeIterStart(bucket: Bucket, key0: Key)
+  lemma noKeyBeforeIterStart(bucket: Bucket, pset: Option<PrefixSet>, key0: Key)
   requires WFBucket(bucket)
   requires BucketWellMarshalled(bucket)
   requires key0 in bucket.as_map()
-  ensures IterStart(bucket).next.Next?
-  ensures Keyspace.lte(IterStart(bucket).next.key, key0)
+  requires pset.Some? ==> IsPrefix(pset.value.prefix, key0)
+  ensures IterStart(bucket, pset).next.Next?
+  ensures Keyspace.lte(IterStart(bucket, pset).next.key, ApplyPrefixSet(pset, key0))
   {
     Keyspace.reveal_IsStrictlySorted();
     reveal_IterStart();
     var i := MapSeqs.GetIndex(bucket.keys, bucket.msgs, key0);
+    var itstart := IterStart(bucket, pset);
+
+    if pset.Some? && itstart.idx < i {
+      var key0' := ApplyPrefixSet(pset, key0);
+      PrefixLteProperties(pset.value.prefix, bucket.keys[itstart.idx], key0);
+      PrefixLteProperties(pset.value.newPrefix, itstart.next.key, key0');
+    }
   }
 
   lemma lemma_NextFromIndex(bucket: Bucket, it: Iterator)
@@ -206,11 +313,13 @@ module BucketIteratorModel {
   ensures 0 <= it.idx <= |bucket.keys|
   ensures 0 <= it.idx < |bucket.keys| ==>
     && it.next.Next?
-    && it.next.key == bucket.keys[it.idx]
+    && (it.pset.Some? ==> IsPrefix(it.pset.value.prefix, bucket.keys[it.idx]))
+    && it.next.key == ApplyPrefixSet(it.pset, bucket.keys[it.idx])
     && it.next.msg == bucket.msgs[it.idx]
   ensures it.idx == |bucket.keys| ==>
     && it.next.Done?
   {
     reveal WFIter();
   }
+
 }
